NLustreToSyMac/Correctness.v
@@ -1,0 +1,230 @@
+Require Import Coq.FSets.FMapPositive.
+Require Import PArith.
+Require Import Velus.Common.
+Require Import Velus.Operators.
+Require Import Velus.Clocks.
+Require Import Velus.NLustre.NLSyntax.
+Require Import Velus.NLustre.Memories.
+Require Import Velus.SyMac.SMSyntax.
+Require Import Velus.NLustre.Ordered.
+Require Import Velus.NLustre.Stream.
+Require Import Velus.NLustre.NLSemantics.
+Require Import Velus.SyMac.SMSemantics.
+Require Import Velus.NLustreToSyMac.Translation.
+
+Require Import List.
+Import List.ListNotations.
+Require Import Coq.Sorting.Permutation.
+Require Import Morphisms.
+
+Open Scope positive.
+Open Scope list.
+
+Module Type CORRECTNESS
+       (Import Ids   : IDS)
+       (Import Op    : OPERATORS)
+       (Import OpAux : OPERATORS_AUX Op)
+       (Import Clks  : CLOCKS      Ids)
+       (Import SynNL : NLSYNTAX    Ids Op       Clks)
+       (SynSM        : SMSYNTAX    Ids Op       Clks)
+       (Import Str   : STREAM          Op OpAux)
+       (Import Ord   : ORDERED     Ids Op       Clks SynNL)
+       (Import SemNL : NLSEMANTICS Ids Op OpAux Clks SynNL       Str Ord)
+       (SemSM        : SMSEMANTICS Ids Op OpAux Clks       SynSM Str)
+       (Import Mem   : MEMORIES    Ids Op       Clks SynNL)
+       (Import Trans : TRANSLATION Ids Op       Clks SynNL SynSM Mem).
+
+  Definition memory_spec (m: SemSM.memory) (mems: list (ident * const)) x :=
+    PS.mem x (ps_from_list (map fst mems)) = true <-> exists lv, RMemory.mfind_mem x m = Some lv.
+
+  Section Global.
+
+    Variable G: SynNL.global.
+    Let P := translate G.
+
+    Section SemInstant.
+
+      Variable base: bool.
+      Variable R: env.
+
+      Lemma var_instant_correctness:
+        forall x v,
+          sem_var_instant R x v ->
+          SemSM.sem_var_instant R x v.
+      Proof.
+        induction 1; constructor; auto.
+      Qed.
+      Hint Resolve var_instant_correctness.
+
+      Lemma clock_instant_correctness:
+        forall ck b,
+          sem_clock_instant base R ck b ->
+          SemSM.sem_clock_instant base R ck b.
+      Proof.
+        induction 1; eauto using SemSM.sem_clock_instant.
+      Qed.
+
+      Lemma typeof_correctness:
+        forall e mems,
+          SynSM.typeof (translate_lexp mems e) = typeof e.
+      Proof.
+        induction e; intros; simpl; auto.
+        destruct (PS.mem i mems); auto.
+      Qed.
+      (* Hint Resolve typeof_correctness. *)
+
+      Variable m: SemSM.memory.
+      Variable mems: list (ident * const).
+      Let memids := ps_from_list (map fst mems).
+
+      Lemma lexp_instant_correctness:
+        forall e b v,
+          sem_lexp_instant base R e v ->
+          SemSM.sem_lexp_instant b base R m 0 mems (translate_lexp memids e) v.
+      Proof.
+        induction 1; simpl; eauto using SemSM.sem_lexp_instant.
+        - destruct (PS.mem x memids) eqn: E.
+          + do 2 constructor.
+            unfold SemSM.get_mem.
+            destruct b.
+            * admit.
+            * admit.
+          + eauto using SemSM.sem_lexp_instant.
+        - econstructor; eauto.
+          now rewrite typeof_correctness.
+        - econstructor; eauto.
+          now rewrite 2 typeof_correctness.
+      Qed.
+      Hint Resolve lexp_instant_correctness.
+
+      Lemma lexps_instant_correctness:
+        forall es b vs,
+          sem_lexps_instant base R es vs ->
+          SemSM.sem_lexps_instant b base R m 0 mems (map (translate_lexp memids) es) vs.
+      Proof.
+        induction 1; constructor; auto.
+      Qed.
+
+      Lemma cexp_instant_correctness:
+        forall ce b v,
+          sem_cexp_instant base R ce v ->
+          SemSM.sem_cexp_instant b base R m 0 mems (translate_cexp memids ce) v.
+      Proof.
+        induction 1; simpl; eauto using SemSM.sem_cexp_instant.
+      Qed.
+
+    End SemInstant.
+    Hint Resolve var_instant_correctness clock_instant_correctness
+         lexp_instant_correctness lexps_instant_correctness
+         cexp_instant_correctness.
+
+    Section Sem.
+
+      Variable bk: stream bool.
+      Variable H: history.
+
+      Lemma var_correctness:
+        forall x xs,
+          sem_var bk H x xs ->
+          SemSM.sem_var H x xs.
+      Proof.
+        intros ** Sem n; specialize (Sem n); auto.
+      Qed.
+      Hint Resolve var_correctness.
+
+      Lemma vars_correctness:
+        forall xs xss,
+          sem_vars bk H xs xss ->
+          SemSM.sem_vars H xs xss.
+      Proof.
+        intros ** Sem n; specialize (Sem n);
+          induction Sem; constructor; auto.
+      Qed.
+
+      Variable M: SemSM.memories.
+      Variable mems: list (ident * const).
+      Let memids := ps_from_list (map fst mems).
+
+      Lemma caexp_correctness:
+        forall ck ce xs,
+          sem_caexp bk H ck ce xs ->
+          SemSM.sem_caexp bk H M 0 mems ck (translate_cexp memids ce) xs.
+      Proof.
+        intros ** Sem n; specialize (Sem n); simpl in Sem.
+        induction Sem; constructor; auto;
+          apply cexp_instant_correctness; auto.
+      Qed.
+
+      Lemma laexps_correctness:
+        forall ck es vs,
+          sem_laexps bk H ck es vs ->
+          SemSM.sem_laexps bk H M 0 mems ck (map (translate_lexp memids) es) vs.
+      Proof.
+        intros ** Sem n; specialize (Sem n); simpl in Sem.
+        induction Sem.
+        - econstructor 1; eauto.
+          now apply lexps_instant_correctness.
+        - constructor; auto.
+          + now rewrite all_absent_map.
+          + now apply lexps_instant_correctness.
+      Qed.
+
+    End Sem.
+    Hint Resolve var_correctness vars_correctness
+         caexp_correctness laexps_correctness.
+
+
+    Theorem correctness:
+      forall f xss oss,
+        sem_node G f xss oss ->
+        exists ma,
+          (forall n, find_node f G = Some n -> ma = translate_node n)
+          /\ exists M, SemSM.sem_mode P 0 ma step M xss oss.
+    Proof.
+      induction 1 as [| | | |???? IHNode|] using sem_node_mult with
+          (P_equation := fun b H e =>
+                           sem_equation G b H e ->
+                           exists M mems,
+                             Forall (SemSM.sem_equation P 0 b H M mems)
+                                    (translate_eqn (ps_from_list (map fst mems)) e))
+          (P_reset := fun f r xss oss =>
+                        sem_reset G f r xss oss ->
+                        True);
+        eauto.
+      - repeat (econstructor; eauto).
+
+      - intro Sem; clear Sem.
+        (* match goal with *)
+        (*   H: sem_node _ _ _ _ |- _ => *)
+        (*   inversion_clear H as [??????? Find] *)
+        (* end. *)
+        destruct IHsem_node as (ma & Spec & M & Sem).
+        match goal with
+          H: sem_node _ _ _ _ |- _ =>
+          inversion_clear H as [??????? Find]
+        end.
+        pose proof Find as Find'.
+        apply Spec in Find'.
+        apply find_node_translate in Find as (ma' & ? & Find & E).
+        subst.
+        (* apply find_node_translate in Find. *)
+        (* destruct Find as (ma' & P' & Find' & E). *)
+
+        simpl.
+        do 2 econstructor.
+        constructor; eauto.
+        econstructor; eauto.
+        +
+          SearchAbout SynSM.find_machine.
+
+
+  sem_det. admit.
+
+      - admit.
+
+      - admit.
+
+      - admit.
+
+      - exists (translate_node n); split; eauto.
+    Qed.
